---
layout: post
title: 2005 AIME I Problems 
tags: math,education,algebra
category: math
---- 

[Source](https://artofproblemsolving.com/wiki/index.php/2009_AIME_II_Problems/Problem_14)

Problem 14
The sequence $(a_n)$ satisfies $a_0=0$ and $a_{n + 1} = \frac{8}{5}a_n + \frac{6}{5}\sqrt{4^n - a_n^2}$ for $n \geq 0$. Find the greatest integer less than or equal to $a_{10}$.

Solution 2
After we do the substitution, we can notice the fact that $\left( \frac 35 \right)^2 + \left( \frac 45 \right)^2 = 1$, which may suggest that the formula may have something to do with the unit circle. Also, the expression $\sqrt{1-x^2}$ often appears in trigonometry, for example in the relationship between the sine and the cosine. Both observations suggest that the formula may have a neat geometric interpretation.

Consider the equation:\[y = \frac45 x + \frac 35\sqrt{1 - x^2}\]

Note that for $t=\sin^{-1} \frac 35$ we have $\sin t=\frac 35$ and $\cos t = \frac 45$. Now suppose that we have $x=\sin s$ for some $s$. Then our equation becomes:

\[y=\cos t \cdot \sin s + \sin t \cdot |\cos s|\]

Depending on the sign of $\cos s$, this is either the angle addition, or the angle subtraction formula for sine. In other words, if $\cos s \geq 0$, then $y=\sin(s+t)$, otherwise $y=\sin(s-t)$.

We have $b_0=0=\sin 0$. Therefore $b_1 = \sin(0+t) = \sin t$, $b_2 = \sin(t+t) = \sin (2t)$, and so on. (Remember that $t$ is the constant defined as $t=\sin^{-1} \frac 35$.)

This process stops at the first $b_k = \sin (kt)$, where $kt$ exceeds $\frac{\pi}2$. Then we'll have $b_{k+1} = \sin(kt - t) = \sin ((k-1)t) = b_{k-1}$ and the sequence will start to oscillate.

Note that $\sin \frac{\pi}6 = \frac 12 < \frac 35$, and $\sin \frac{\pi}4 = \frac{\sqrt 2}2 > \frac 35$, hence $t$ is strictly between $\frac{\pi}6$ and $\frac{\pi}4$. Then $2t\in\left(\frac{\pi}3,\frac{\pi}2 \right)$, and $3t\in\left( \frac{\pi}2, \frac{3\pi}4 \right)$. Therefore surely $2t < \frac{\pi}2 < 3t$.

Hence the process stops with $b_3 = \sin (3t)$, we then have $b_4 = \sin (2t) = b_2$. As in the previous solution, we conclude that $b_{10}=b_2$, and that the answer is $\lfloor a_{10} \rfloor  = \left\lfloor 2^{10} b_{10} \right\rfloor = \boxed{983}$.