---
layout: post
title: 加拿大奥赛题
tags: math,education,algebra
category: math
---

> [Source](https://www.bilibili.com/video/BV1WZS1YvEt8?spm_id_from=333.788.recommend_more_video.2&vd_source=2c3b1cf87d67c244536d57d4d5b68285)

计算

$$
    \sum_{n=1}^{1994} (-1)^n \frac{n^2 + n + 1}{n!}
$$

***Solution***

注意到 $n^2 +n + 1 = n(n-1) + 2n + 1$，原题简化为（取$m = 1994$）

> 注意求和下标的变换

$$
\begin{aligned}
    &\sum_{n=1}^{m} (-1)^n \frac{n^2 + n + 1}{n!} \\
    &= \sum_{n=1}^{m} (-1)^n \frac{n(n-1) + 2n + 1}{n!} \\
    &= 
        \sum_{n=1}^{m} (-1)^n \frac{n(n-1)}{n!} + 
        \sum_{n=1}^{m} (-1)^n \frac{2n}{n!} + 
        \sum_{n=1}^{m} (-1)^n \frac{1}{n!} \\
    &= 
        \sum_{n=2}^{m} (-1)^{n-2} \frac{1}{(n-2)!} 
        - 2 \sum_{n=1}^{m} (-1)^{n-1} \frac{1}{(n-1)!} + 
        \sum_{n=1}^{m} (-1)^n \frac{1}{n!} \\
    &= 
        \sum_{k=0}^{m-2} (-1)^k \frac{1}{k!}
        - 2 \sum_{k=0}^{m-1} (-1)^k \frac{1}{k!} + 
        \sum_{k=1}^{m} (-1)^k \frac{1}{k!} \\
    &= 
        \sum_{k \in \{0\}} (-1)^k \frac{1}{k!}
        - 2 \sum_{k \in \{0, m-1\}} (-1)^k \frac{1}{k!} + 
        \sum_{k \in \{ m-1, m \}} (-1)^k \frac{1}{k!} \\
    &= 
        1 - 2 -  (-1)^{m-1}\frac{1}{(m-1)!}
        + (-1)^m \frac{1}{m!} \\
    & = (-1)^m \cdot \frac{(m + 1)}{m!} - 1 \\
    &= \frac{1995}{1994!} - 1
\end{aligned}
$$